TriInv.fst
@@ -10,13 +10,11 @@ open Identity
 #push-options "--split_queries always"
 let rec triangular_inv (#n:pos) (l:unit_lower n)
     : r:unit_lower n { is_inverse l r } =
-  match n with
-  | 1 ->
-      one_by_one_is_identity l;
-      l
-  | _ ->
-      let c, o, l' = destruct_lower l in
-      let l'_inv = triangular_inv l' in
-      let b = neg (mat_vec_mul l'_inv c) in
-    augment_lower l'_inv b one_const
+    match n with
+    | 1 -> l
+    | _ ->
+        let c, o, l' = destruct_lower l in
+        let l'_inv = triangular_inv l' in
+        let b = neg (mat_vec_mul l'_inv c) in
+        augment_lower l'_inv b one_const
 #pop-options
